byteback-whyml/src/main/java/byteback/mlcfg/IOC.java
@@ -1,11 +1,15 @@
 package byteback.mlcfg;
 
 import byteback.mlcfg.printer.RecordPrinter;
+import byteback.mlcfg.syntax.identifiers.IdentifierEscaper;
+import byteback.mlcfg.vimpParser.TypeResolver;
 import byteback.mlcfg.vimpParser.VimpClassParser;
 
 public final class IOC {
-    public static final VimpClassParser classParser = new VimpClassParser();
-    public static final RecordPrinter recordPrinter = new RecordPrinter();
+    public static final IdentifierEscaper identifierEscaper = new IdentifierEscaper();
+    public static final TypeResolver typeResolver = new TypeResolver(identifierEscaper);
+    public static final VimpClassParser classParser = new VimpClassParser(typeResolver);
+    public static final RecordPrinter recordPrinter = new RecordPrinter(identifierEscaper);
     public static final ProgramConverter programConverter = new ProgramConverter(classParser, recordPrinter);
     private IOC() {
     }
