byteback-whyml/src/main/java/byteback/mlcfg/printer/RecordPrinter.java
@@ -1,13 +1,28 @@
 package byteback.mlcfg.printer;
 
-import byteback.mlcfg.syntax.RecordDeclaration;
+import byteback.mlcfg.syntax.WhyRecordDeclaration;
 
+import byteback.mlcfg.syntax.identifiers.IdentifierEscaper;
 import java.util.stream.Collectors;
 
 public class RecordPrinter {
-    public String printRecord(final RecordDeclaration r) {
+    private final IdentifierEscaper identifierEscaper;
+
+	public RecordPrinter(IdentifierEscaper identifierEscaper) {
+		this.identifierEscaper = identifierEscaper;
+	}
+
+    public String printRecord(final WhyRecordDeclaration r) {
         return r.fields().stream()
-                .map(f -> String.format("  %s: %s", f.name(), f.type()))
-                .collect(Collectors.joining(";\n", String.format("type %s = {\n", r.name()), "\n}"));
+                .map(f -> String.format(
+						"  %s: %s",
+						identifierEscaper.escape(f.name()),
+						f.type().getPrefix().map(s -> s + " ").orElse("") + f.type().getIdentifier()))
+                .collect(Collectors.joining(
+						";\n",
+						String.format(
+								"type %s = {\n",
+								identifierEscaper.escape(r.name())),
+						"\n}"));
     }
 }
