byteback-whyml/src/main/java/byteback/mlcfg/syntax/RecordDeclaration.java
@@ -1,7 +1,0 @@
-package byteback.mlcfg.syntax;
-
-import java.util.List;
-
-public record RecordDeclaration(String name, List<RecordFieldDeclaration> fields) {
-
-}
