byteback-whyml/src/main/java/byteback/mlcfg/syntax/RecordFieldDeclaration.java
@@ -1,4 +1,0 @@
-package byteback.mlcfg.syntax;
-
-public record RecordFieldDeclaration(String name, String type) {
-}
