byteback-whyml/src/main/java/byteback/mlcfg/syntax/WhyProgram.java
@@ -2,7 +2,7 @@ package byteback.mlcfg.syntax;
 
 import byteback.frontend.boogie.ast.Printable;
 
-public record Program(String program) implements Printable {
+public record WhyProgram(String program) implements Printable {
     @Override
     public void print(StringBuilder builder) {
         builder.append(program).append('\n');
