byteback-whyml/src/main/java/byteback/mlcfg/syntax/WhyRecordDeclaration.java
@@ -1,0 +1,7 @@
+package byteback.mlcfg.syntax;
+
+import java.util.List;
+
+public record WhyRecordDeclaration(String name, List<WhyRecordFieldDeclaration> fields) {
+
+}
