byteback-whyml/src/main/java/byteback/mlcfg/syntax/WhyRecordFieldDeclaration.java
@@ -1,0 +1,6 @@
+package byteback.mlcfg.syntax;
+
+import byteback.mlcfg.syntax.types.WhyType;
+
+public record WhyRecordFieldDeclaration(String name, WhyType type) {
+}
