byteback-whyml/src/main/java/byteback/mlcfg/syntax/identifiers/IdentifierEscaper.java
@@ -1,0 +1,17 @@
+package byteback.mlcfg.syntax.identifiers;
+
+import java.util.stream.Collectors;
+
+public class IdentifierEscaper {
+	public String escape(String input) {
+		return input.codePoints().mapToObj(e -> {
+			if (Character.isLetterOrDigit(e)) {
+				return Character.toString(e);
+			} else if (e == '_') {
+				return "__"; // underscores are doubled
+			} else {
+				return String.format("_u%04X", e); // all other characters are encoded as unicode codepoints
+			}
+		}).collect(Collectors.joining(""));
+	}
+}
