byteback-whyml/src/main/java/byteback/mlcfg/syntax/types/WhyArrayType.java
@@ -1,0 +1,23 @@
+package byteback.mlcfg.syntax.types;
+
+import java.util.Optional;
+import java.util.stream.Collectors;
+import java.util.stream.Stream;
+
+public class WhyArrayType implements WhyType {
+	private final WhyType baseType;
+
+	public WhyArrayType(WhyType baseType) {
+		this.baseType = baseType;
+	}
+
+	@Override
+	public Optional<String> getPrefix() {
+		return Optional.of("array");
+	}
+
+	@Override
+	public String getIdentifier() {
+		return baseType.getPrefix().map(s -> s + " ").orElse("") + baseType.getIdentifier();
+	}
+}
