byteback-whyml/src/main/java/byteback/mlcfg/syntax/types/WhyPrimitive.java
@@ -1,0 +1,41 @@
+package byteback.mlcfg.syntax.types;
+
+import java.util.Optional;
+
+public enum WhyPrimitive implements WhyType {
+	/**
+	 * "true" or "false"
+	 */
+	BOOL("bool"),
+
+	/**
+	 * An unbounded integer type
+	 */
+	INT_INT("int.Int"), // TODO: consider bounded integer types for all JVM primitive types
+
+	/**
+	 * IEEE 754 single precision
+	 */
+	FLOAT_8_23("<float 8 23>"),
+
+	/**
+	 * IEEE 754 double precision
+	 */
+	FLOAT_11_52("<float 11 52>");
+
+	private final String label;
+
+	WhyPrimitive(String typeLabel) {
+		this.label = typeLabel;
+	}
+
+	@Override
+	public Optional<String> getPrefix() {
+		return Optional.empty();
+	}
+
+	@Override
+	public String getIdentifier() {
+		return label;
+	}
+}
