byteback-whyml/src/main/java/byteback/mlcfg/syntax/types/WhyReference.java
@@ -1,0 +1,22 @@
+package byteback.mlcfg.syntax.types;
+
+import java.util.Optional;
+
+// TODO: using references here is wrong. We need to implement a heap model
+public class WhyReference implements WhyType {
+	private final String className;
+
+	public WhyReference(String className) {
+		this.className = className;
+	}
+
+	@Override
+	public Optional<String> getPrefix() {
+		return Optional.of("ref");
+	}
+
+	@Override
+	public String getIdentifier() {
+		return className;
+	}
+}
