byteback-whyml/src/main/java/byteback/mlcfg/syntax/types/WhyType.java
@@ -1,0 +1,8 @@
+package byteback.mlcfg.syntax.types;
+
+import java.util.Optional;
+
+public interface WhyType {
+	Optional<String> getPrefix();
+	String getIdentifier();
+}
