byteback-whyml/src/main/java/byteback/mlcfg/vimpParser/TypeAccessExtractor.java
@@ -1,0 +1,97 @@
+package byteback.mlcfg.vimpParser;
+
+import byteback.analysis.TypeSwitch;
+import byteback.mlcfg.syntax.identifiers.IdentifierEscaper;
+import byteback.mlcfg.syntax.types.WhyArrayType;
+import byteback.mlcfg.syntax.types.WhyPrimitive;
+import byteback.mlcfg.syntax.types.WhyReference;
+import byteback.mlcfg.syntax.types.WhyType;
+import soot.ArrayType;
+import soot.BooleanType;
+import soot.ByteType;
+import soot.CharType;
+import soot.DoubleType;
+import soot.FloatType;
+import soot.IntType;
+import soot.LongType;
+import soot.RefType;
+import soot.ShortType;
+import soot.Type;
+
+public class TypeAccessExtractor extends TypeSwitch<WhyType> {
+
+	private final IdentifierEscaper escaper;
+
+	private WhyType type;
+
+	public TypeAccessExtractor(IdentifierEscaper escaper) {
+		this.escaper = escaper;
+	}
+
+	@Override
+	public void caseByteType(final ByteType byteType) {
+		type = WhyPrimitive.INT_INT;
+	}
+
+	@Override
+	public void caseShortType(final ShortType shortType) {
+		type = WhyPrimitive.INT_INT;
+	}
+
+	@Override
+	public void caseIntType(final IntType integerType) {
+		type = WhyPrimitive.INT_INT;
+	}
+
+	@Override
+	public void caseCharType(final CharType charType) {
+		type = WhyPrimitive.INT_INT;
+	}
+
+	@Override
+	public void caseLongType(final LongType longType) {
+		type = WhyPrimitive.INT_INT;
+	}
+
+	@Override
+	public void caseDoubleType(final DoubleType doubleType) {
+		type = WhyPrimitive.FLOAT_11_52;
+	}
+
+	@Override
+	public void caseFloatType(final FloatType floatType) {
+		type = WhyPrimitive.FLOAT_8_23;
+	}
+
+	@Override
+	public void caseBooleanType(final BooleanType booleanType) {
+		type = WhyPrimitive.BOOL;
+	}
+
+	@Override
+	public void caseRefType(final RefType referenceType) {
+		type = new WhyReference(escaper.escape(referenceType.getClassName()));
+	}
+
+	@Override
+	public void caseArrayType(final ArrayType arrayType) {
+		// TODO: consider rewriting this
+		final TypeAccessExtractor e = new TypeAccessExtractor(escaper);
+		e.visit(arrayType.getElementType());
+		type = new WhyArrayType(e.result());
+	}
+
+	@Override
+	public void caseDefault(final Type type) {
+		throw new IllegalStateException("Cannot extract type access for type " + type);
+	}
+
+	@Override
+	public WhyType result() {
+		if (type == null) {
+			throw new IllegalStateException("Could not retrieve type access");
+		}
+
+		return type;
+	}
+}
