byteback-whyml/src/main/java/byteback/mlcfg/vimpParser/TypeResolver.java
@@ -1,0 +1,20 @@
+package byteback.mlcfg.vimpParser;
+
+import byteback.mlcfg.syntax.identifiers.IdentifierEscaper;
+import byteback.mlcfg.syntax.types.WhyType;
+import soot.Type;
+
+public class TypeResolver {
+
+	private final IdentifierEscaper escaper;
+
+	public TypeResolver(IdentifierEscaper escaper) {
+		this.escaper = escaper;
+	}
+
+	public WhyType resolveType(Type sootType) {
+		final TypeAccessExtractor e = new TypeAccessExtractor(escaper);
+		e.visit(sootType);
+		return e.result();
+	}
+}
