byteback-whyml/src/main/java/byteback/mlcfg/vimpParser/VimpClassParser.java
@@ -1,17 +1,37 @@
 package byteback.mlcfg.vimpParser;
 
-import byteback.mlcfg.syntax.RecordDeclaration;
-import byteback.mlcfg.syntax.RecordFieldDeclaration;
-import soot.SootClass;
-
+import byteback.mlcfg.syntax.WhyRecordDeclaration;
+import byteback.mlcfg.syntax.WhyRecordFieldDeclaration;
 import java.util.List;
+import java.util.stream.Stream;
+import soot.SootClass;
+import soot.SootField;
 
 public class VimpClassParser {
-    public RecordDeclaration parseClassDeclaration(SootClass clazz) {
-        final String className = clazz.getName();
-        final List<RecordFieldDeclaration> fields = clazz.getFields().stream()
-                .map(f -> new RecordFieldDeclaration(f.getName(), f.getType().toQuotedString()))
-                .toList();
-        return new RecordDeclaration(className, fields);
-    }
+
+	private final TypeResolver typeResolver;
+
+	public VimpClassParser(TypeResolver typeResolver) {
+		this.typeResolver = typeResolver;
+	}
+
+	private List<WhyRecordFieldDeclaration> toFieldDeclarationList(Stream<SootField> fields) {
+		return fields.map(f -> new WhyRecordFieldDeclaration(f.getName(), typeResolver.resolveType(f.getType())))
+				.toList();
+	}
+
+	public Stream<WhyRecordDeclaration> parseClassDeclaration(SootClass clazz) {
+		final String className = clazz.getName();
+
+		final List<WhyRecordFieldDeclaration> instanceFields =
+				toFieldDeclarationList(clazz.getFields().stream().filter(e -> !e.isStatic()));
+
+		final List<WhyRecordFieldDeclaration> staticFields =
+				toFieldDeclarationList(clazz.getFields().stream().filter(SootField::isStatic));
+
+		return Stream.of(
+				new WhyRecordDeclaration("instance_" + className, instanceFields),
+				new WhyRecordDeclaration("static_" + className, staticFields)
+		).filter(e -> !e.fields().isEmpty());
+	}
 }
